test.lean
@@ -6,6 +6,7 @@
 
 import Tests.TestMain
 import Tests.TestComplexity
+import Tests.TestLiteralsExpr
 import LeanC.Arrays
 
 open Lean IO
@@ -24,4 +25,4 @@ def runAll (runners : List (IO UInt32)) : IO UInt32 := do
 def main : IO UInt32 := do
   -- Add each test module's `main` here in the same order as imports above.
   -- Expand this list when new tests are added under `tests/`.
-  runAll [TestMain.test, TestComplexity.test]
+  runAll [TestMain.test, TestComplexity.test, TestLiteralsExpr.test]
